src/Semantics.v
@@ -4,6 +4,28 @@ Require Import Coq.Strings.String.
 Require Import Ast.
 Require Import Store.
 
+Definition addr := nat.
+Module addr_eq.
+  Definition t := addr.
+  Definition eqb x y : bool := beq_nat x y.
+End addr_eq.
+
+Definition object := string.
+Definition actor := string.
+
+Module heap_default.
+  Definition t : Type := actor + object.
+  Definition default : t := inl EmptyString.
+End heap_default.
+
+Module Heap.
+  Include Store addr_eq heap_default.
+  Definition alloc_addr (st: store) : addr :=
+    List.length st.
+End Heap.
+
+Definition heap := Heap.store.
+
 Inductive local_id : Type :=
 | SourceId: string -> local_id
 | TempId: nat -> local_id.
@@ -20,13 +42,12 @@ End local_id_eq.
 
 Inductive value : Type :=
 | v_null: value
-| v_addr: nat -> value.
+| v_addr: addr -> value.
 
 Module value_default.
   Definition t := value.
   Definition default := v_null.
 End value_default.
-
 
 Module Frame.
   Include Store local_id_eq value_default.
@@ -36,91 +57,92 @@ End Frame.
 
 Definition frame := Frame.store.
 
-Reserved Notation "f1 / e1 '==>' f2 / e2"
-  (at level 40, e1 at level 39, f2 at level 39).
+Reserved Notation "h1 / f1 / e1 '==>' h2 / f2 / e2"
+  (at level 40, e1 at level 39, h2 at level 39, f1 at level 38, f2 at level 38).
 
-Inductive step : frame * expr -> frame * expr -> Prop :=
-| E_Seq : forall f t e,
-    f / expr_seq (expr_temp t) e ==> f / e
+Inductive step : heap * frame * expr -> heap * frame * expr -> Prop :=
+| E_Seq : forall h f t e,
+    h / f / expr_seq (expr_temp t) e ==> h / f / e
 
-| E_Recover : forall f t,
-    f / expr_recover (expr_temp t) ==> f / (expr_temp t)
+| E_Recover : forall h f t,
+    h / f / expr_recover (expr_temp t) ==> h / f / (expr_temp t)
 
-| E_Local : forall f t f' name,
+| E_Local : forall h f t f' name,
     t = Frame.alloc_temp f ->
     f' = Frame.set f (TempId t) (Frame.get f (SourceId name)) ->
-    f / expr_local name ==> f' / expr_temp t
+    h / f / expr_local name ==> h / f' / expr_temp t
 
-| E_Asn_Local : forall f f' t t' name,
+| E_Asn_Local : forall h f f' t t' name,
     t' = Frame.alloc_temp f ->
     f' = Frame.set (Frame.set f (TempId t') (Frame.get f (SourceId name)))
               (SourceId name) (Frame.get f (TempId t)) ->
-    f / expr_assign_local name (expr_temp t) ==> f' / expr_temp t'
+    h / f / expr_assign_local name (expr_temp t) ==> h / f' / expr_temp t'
 
-| E_Seq1 : forall f f' e1 e1' e2,
-    f / e1 ==> f' / e1' ->
-    f / expr_seq e1 e2 ==> f' / expr_seq e1' e2
+| E_Seq1 : forall h f f' e1 e1' e2,
+    h / f / e1 ==> h / f' / e1' ->
+    h / f / expr_seq e1 e2 ==> h / f' / expr_seq e1' e2
 
-| E_Recover1 : forall f f' e e',
-    f / e ==> f' / e' ->
-    f / expr_recover e ==> f' / expr_recover e'
+| E_Recover1 : forall h f f' e e',
+    h / f / e ==> h / f' / e' ->
+    h / f / expr_recover e ==> h / f' / expr_recover e'
 
-| E_Asn_Local1 : forall f f' name e e',
-    f / e ==> f' / e' ->
-    f / expr_assign_local name e ==> f' / expr_assign_local name e'
+| E_Asn_Local1 : forall h f f' name e e',
+    h / f / e ==> h / f' / e' ->
+    h / f / expr_assign_local name e ==> h / f' / expr_assign_local name e'
 
-where "f1 / e1 '==>' f2 / e2" := (step (f1,e1) (f2,e2)).
+where "h1 / f1 / e1 '==>' h2 / f2 / e2" := (step (h1,f1,e1) (h2,f2,e2)).
 
-Reserved Notation "f1 / e1 '==>*' f2 / e2"
-  (at level 40, e1 at level 39, f2 at level 39).
+Reserved Notation "h1 / f1 / e1 '==>*' h2 / f2 / e2"
+  (at level 40, e1 at level 39, h2 at level 39, f1 at level 38, f2 at level 38).
 
-Inductive multistep : frame * expr -> frame * expr -> Prop :=
-| multi_refl : forall f e, multistep (f, e) (f, e)
+Inductive multistep : heap * frame * expr -> heap * frame * expr -> Prop :=
+| multi_refl : forall h f e, multistep (h, f, e) (h, f, e)
 
-| multi_trans : forall f1 e1 f2 e2 f3 e3,
-    f1 / e1 ==> f2 / e2 ->
-    f2 / e2 ==>* f3 / e3 ->
-    f1 / e1 ==>* f3 / e3
-where "f1 / e1 '==>*' f2 / e2" := (multistep (f1, e1) (f2, e2)).
+| multi_trans : forall h1 f1 e1 h2 f2 e2 h3 f3 e3,
+    h1 / f1 / e1 ==> h2 / f2 / e2 ->
+    h2 / f2 / e2 ==>* h3 / f3 / e3 ->
+    h1 / f1 / e1 ==>* h3 / f3 / e3
+where "h1 / f1 / e1 '==>*' h2 / f2 / e2" := (multistep (h1, f1, e1) (h2, f2, e2)).
 
-Theorem multi_one : forall f1 e1 f2 e2,
-  f1 / e1 ==> f2 / e2 ->
-  f1 / e1 ==>* f2 / e2.
+Theorem multi_one : forall h1 f1 e1 h2 f2 e2,
+  h1 / f1 / e1 ==> h2 / f2 / e2 ->
+  h1 / f1 / e1 ==>* h2 / f2 / e2.
 Proof.
 intros.
-apply multi_trans with (f2 := f2) (e2 := e2).
+apply multi_trans with (h2 := h2) (f2 := f2) (e2 := e2).
 exact H.
 apply multi_refl.
 Qed.
 
-Theorem multi_concat : forall f1 e1 f2 e2 f3 e3,
-  f1 / e1 ==>* f2 / e2 ->
-  f2 / e2 ==>* f3 / e3 ->
-  f1 / e1 ==>* f3 / e3.
+Theorem multi_concat : forall h1 f1 e1 h2 f2 e2 h3 f3 e3,
+  h1 / f1 / e1 ==>* h2 / f2 / e2 ->
+  h2 / f2 / e2 ==>* h3 / f3 / e3 ->
+  h1 / f1 / e1 ==>* h3 / f3 / e3.
 Proof.
   intros.
+  generalize dependent h3.
   generalize dependent f3.
   generalize dependent e3.
   induction H.
   + intros. exact H0.
   + intros.
-    apply multi_trans with (f2 := f3) (e2 := e3).
+    apply multi_trans with (h2 := h3) (f2 := f3) (e2 := e3).
     exact H.
     apply IHmultistep.
     exact H1.
 Qed.
 
-Lemma E_RecoverN : forall f f' e e',
-    f / e ==>* f' / e' ->
-    f / expr_recover e ==>* f' / expr_recover e'.
+Lemma E_RecoverN : forall h h' f f' e e',
+    h / f / e ==>* h' / f' / e' ->
+    h / f / expr_recover e ==>* h' / f' / expr_recover e'.
 Admitted.
 
-Lemma E_SeqN : forall f f' e1 e1' e2,
-    f / e1 ==>* f' / e1' ->
-    f / expr_seq e1 e2 ==>* f' / expr_seq e1' e2.
+Lemma E_SeqN : forall h h' f f' e1 e1' e2,
+    h / f / e1 ==>* h' / f' / e1' ->
+    h / f / expr_seq e1 e2 ==>* h' / f' / expr_seq e1' e2.
 Admitted.
 
-Lemma E_Asn_LocalN : forall f f' name e e',
-    f / e ==>* f' / e' ->
-    f / expr_assign_local name e ==>* f' / expr_assign_local name e'.
+Lemma E_Asn_LocalN : forall h h' f f' name e e',
+    h / f / e ==>* h' / f' / e' ->
+    h / f / expr_assign_local name e ==>* h' / f' / expr_assign_local name e'.
 Admitted.
